### Notes and Scratch Work

```
n = Total length of word
v = Number of vowels in word

aba
    a   1
    b   0
    a   1
    ab  1
    ba  1
    aba 2

This is the same as doing "aaaa" instead of "aba" --> becomes 4 choose 2 = 6

abc
    a   1
    b   0
    c   0
    ab  1
    bc  0
    abc 1

    abc -> aaa -> 3 choose 1 = 3

abba
    a       1
    b       0
    b       0
    a       1

    ab      1
    bb      0
    ba      1

    abb     1
    bba     1

    abba    2

    Total: (1)+(1+1)+(1+1+1)+(2) = 8
    abba --> aaaba --> aaaaaa --> 6 choose 2 = 15 WRONG
    abba -> aaba --> aaaaa -> 5 choose 2 = 10 WRONG
    abba -> aaaa --> 4 choose 2 = 6 WRONG

    contributions:
    a   4
    b   0
    b   0
    a   4

abab
    a       1
    b       0
    a       1
    b       0

    ab      1
    ba      1
    ab      1

    aba     2
    bab     1

    abab    2

    Total = 2+3+3+2 = 10

    contributions:
    a   4 = 0 * 3 + 4
    b   0
    a   6 = (left * right) + total string length = 2 * 1 + 4
    b   0

```

**Realization**: Each vowel contributes the following to the output:

$$(\text{characters left}) * (\text{characters right}) + \text{word length}$$
